A math file about why online softmax works

src/lib/kuiper/Kuiper.Real.fst
@@ -76,6 +76,17 @@ let log_div (x y : real{x >. 0.0R /\ y >. 0.0R})
     assert (rexp (rlog x -. rlog y) == rexp (rlog x) /. rexp (rlog y));
     ()
 
+let rsum_append (s1 s2 : Seq.seq real)
+  : Lemma (ensures rsum (s1 @+ s2) == rsum s1 +. rsum s2)
+          [SMTPat (rsum (s1 @+ s2))]
+  = calc (==) {
+      rsum (s1 @+ s2);
+      == {}
+      seq_fold_left (+.) 0.0R (s1 @+ s2);
+      == { lemma_seq_fold_left_sum 0.0R (+.) s1 s2 }
+      seq_fold_left (+.) 0.0R s1 +. seq_fold_left (+.) 0.0R s2;
+    }
+
 let rec sum_non_zero
     (s : Seq.seq real { forall (i:natlt (Seq.length s)). Seq.index s i >. 0.0R })
     (acc : real)
